More assembly equivalence WIP (#1109)
Only two subgoals remain:
```coq
  R_runtime_output frame runtime_rets
    (type_spec_of_runtime (word_args_to_Z_args word_runtime_inputs))
    (Datatypes.length x) stack_base asm_args_out asm_args_in callee_saved_registers
    runtime_callee_saved_registers m'
```
and
```coq
 R
   (frame ⋆ R_list_scalar_or_array x0 asm_args_out
    ⋆ R_list_scalar_or_array (word_args_to_Z_args word_runtime_inputs)
        asm_args_in ⋆ array cell64 (word.of_Z 8) stack_base x)%sep x1
   (update_dag_with (init_symbolic_state d) (fun _ : dag => d0)) m
 ->
 R_mem frame G_final dag_state1
   (rev (List.combine x4 x5) ++
    rev
      (flat_map
         (fun pat : (idx + idx * list idx) * (idx + list idx) =>
          match pat with
          | (inl _, _) => []
          | (inr (_, addrs'), inl _) => []
          | (inr (_, addrs'), inr items) => List.combine addrs' items
          end) (List.combine x3 (l4 ++ inputs))) ++ init_symbolic_state d) m
```

The first goal is that we must connect everything from the final
symbolic evaluation with our output spec.

The second goal is that we must connect the memory predicate from before
SymexLines (post-initialization) with the desired memory predicate, by
showing that we've updated symbolic memory as desired.

Note that we'll probably want some `iff` statements around `R_mem`,
because what we do in one direction in the first goal we do in the other
direction in the second goal.

src/Assembly/WithBedrock/Proofs.v
@@ -2,6 +2,7 @@ Require Import Coq.Lists.List.
 Require Import Coq.micromega.Lia.
 Require Import Coq.NArith.NArith.
 Require Import Coq.ZArith.ZArith.
+Require Import Coq.Classes.Morphisms.
 Require Import Crypto.Language.PreExtra.
 Require Import Crypto.Language.API.
 Require Import Crypto.Language.APINotations.
@@ -1666,7 +1667,10 @@ Lemma GetReg_ok G s s' reg idx rn lo sz v
       (m' := s'.(symbolic_mem_state))
       (Hd : gensym_dag_ok G d)
       (Hr : forall idx', get_reg r rn = Some idx' -> eval_idx_Z G d idx' v)
-  : (eval_idx_Z G d' idx (Z.land v (Z.ones 64))
+  : ((exists idx',
+         get_reg r rn = Some idx'
+         /\ eval_idx_Z G d idx' v)
+     /\ eval_idx_Z G d' idx (Z.land v (Z.ones 64))
      /\ r = r'
      /\ f = f'
      /\ m = m')
@@ -1723,14 +1727,17 @@ Lemma GetReg_ok_bounded G s s' reg idx rn lo sz v
       (Hd : gensym_dag_ok G d)
       (Hr : forall idx', get_reg r rn = Some idx' -> eval_idx_Z G d idx' v)
       (Hv : (0 <= v < 2^64)%Z)
-  : (eval_idx_Z G d' idx v
+  : ((exists idx',
+         get_reg r rn = Some idx'
+         /\ eval_idx_Z G d idx' v)
+     /\ eval_idx_Z G d' idx v
      /\ r = r'
      /\ f = f'
      /\ m = m')
     /\ gensym_dag_ok G d'
     /\ (forall e n, eval G d e n -> eval G d' e n).
 Proof.
-  replace v with (Z.land v (Z.ones (Z.of_N 64))); [ eapply GetReg_ok; eassumption | rewrite land_ones_eq_of_bounded by assumption ].
+  replace v with (Z.land v (Z.ones (Z.of_N 64))) at 1; [ eapply GetReg_ok; eassumption | rewrite land_ones_eq_of_bounded by assumption ].
   reflexivity.
 Qed.
 
@@ -2651,8 +2658,12 @@ Lemma mapM_GetReg_ok_bounded G
            (Hd : gensym_dag_ok G d)
            (Hwide : Forall (fun reg => let '(_, _, sz) := index_and_shift_and_bitcount_of_reg reg in sz = 64%N) regs)
            (Hbounded : Forall (fun v => (0 <= v < 2^64)%Z) reg_vals)
-           (Hregval : Forall2 (option_eq (eval_idx_Z G s)) (List.map (get_reg r) (List.map reg_index regs)) (List.map Some reg_vals)),
-    (Forall2 (eval_idx_Z G s') idxs reg_vals
+           (Hregval_len : List.length regs = List.length reg_vals)
+           (Hregval : Forall2 (fun idx v => forall idx', idx = Some idx' -> eval_idx_Z G s idx' v) (List.map (get_reg r) (List.map reg_index regs)) reg_vals),
+    ((exists reg_idxs,
+         List.map (get_reg r) (List.map reg_index regs) = List.map Some reg_idxs
+         /\ Forall2 (eval_idx_Z G s') reg_idxs reg_vals)
+     /\ Forall2 (eval_idx_Z G s') idxs reg_vals
      /\ r = r'
      /\ f = f'
      /\ m = m')
@@ -2663,9 +2674,10 @@ Proof.
       idxs as [|idx idxs],
         reg_vals as [|reg_val reg_vals];
     try specialize (IH idxs reg_vals).
-  all: repeat first [ progress cbn [mapM List.map fst snd Symbolic.dag_state Symbolic.symbolic_reg_state Symbolic.symbolic_mem_state Symbolic.symbolic_flag_state] in *
+  all: repeat first [ progress cbn [mapM List.map fst snd Symbolic.dag_state Symbolic.symbolic_reg_state Symbolic.symbolic_mem_state Symbolic.symbolic_flag_state List.length] in *
                     | progress cbv [Symbolic.ret Symbolic.bind ErrorT.bind] in *
                     | progress intros
+                    | progress destruct_head'_ex
                     | progress destruct_head'_prod
                     | progress destruct_head'_and
                     | progress inversion_option
@@ -2673,15 +2685,22 @@ Proof.
                     | progress inversion_prod
                     | progress subst
                     | progress inversion_list
+                    | progress inversion_nat_eq
                     | progress specialize_by_assumption
                     | progress destruct_head' symbolic_state
                     | progress specialize_by (eapply Forall2_weaken; [ | eassumption ]; cbv [option_eq]; intros *; break_innermost_match; eauto using lift_eval_idx_Z_impl)
+                    | exfalso; lia
                     | match goal with
                       | [ H : Forall2 _ (_ :: _) _ |- _ ] => inversion H; clear H
                       | [ H : Forall2 _ [] _ |- _ ] => inversion H; clear H
                       | [ H : Forall _ (_ :: _) |- _ ] => inversion H; clear H
+                      | [ |- exists reg_idxs, _ :: _ = List.map Some reg_idxs /\ _ ]
+                        => eexists (_ :: _); cbn [List.map]; split; [ apply f_equal2; eassumption | ]
                       | [ IH : forall s s', mapM ?f ?ls s = Success (?v, s') -> _, H : mapM ?f ?ls _ = Success (?v, _) |- _ ]
                         => specialize (IH _ _ H)
+                      | [ H : forall ls, nil = List.map _ ls -> _ |- _ ]
+                        => specialize (H nil eq_refl)
+                      | [ |- exists ls, nil = List.map _ ls /\ _ ] => exists nil
                       | [ H : get_reg ?r ?ri = Some ?i, H' : eval_idx_Z ?G ?d ?i ?v |- _ ]
                         => unique assert (forall i', get_reg r ri = Some i' -> eval_idx_Z G d i' v)
                           by now intro; rewrite H; inversion 1; subst; assumption
@@ -2691,7 +2710,8 @@ Proof.
                       | [ |- Forall2 _ (_ :: _) (_ :: _) ] => constructor
                       end
                     | solve [ eauto 10 using lift_eval_idx_Z_impl ]
-                    | break_innermost_match_hyps_step ].
+                    | break_innermost_match_hyps_step
+                    | apply conj; eauto 10 using lift_eval_idx_Z_impl; [] ].
 Qed.
 
 Import Map.Interface Map.Separation. (* for coercions *)
@@ -2838,7 +2858,7 @@ Lemma init_symbolic_state_G_ok m G d G' ss
       (Hframe : frame m)
       (Hbounds : Forall (fun v => (0 <= v < 2^64)%Z) (Tuple.to_list 16 m.(machine_reg_state)))
   : R frame G' ss m
-    /\ (forall regs, Forall (fun v => Option.is_Some v = true) (List.map (get_reg ss.(symbolic_reg_state)) (List.map reg_index regs)))
+    /\ (forall reg, Option.is_Some (get_reg ss.(symbolic_reg_state) (reg_index reg)) = true)
     /\ gensym_dag_ok G' d'
     /\ (forall e n, eval G d e n -> eval G' d' e n).
 Proof.
@@ -2850,7 +2870,6 @@ Proof.
   2: { cbv [Tuple.repeat R_flags Tuple.append Tuple.fieldwise Tuple.fieldwise' R_flag]; cbn [fst snd];
        repeat apply conj; congruence. }
   2: { intros; cbn [List.map]; cbv [get_reg symbolic_reg_state].
-       rewrite !Forall_map, Forall_forall; intros.
        unshelve erewrite <- Tuple.nth_default_to_list, Tuple.from_list_default_eq, Tuple.to_list_from_list.
        { rewrite map_length.
          erewrite length_Forall2, Tuple.length_to_list
@@ -2887,7 +2906,7 @@ Lemma init_symbolic_state_ok m G d
       (Hframe : frame m)
   : exists G',
     R frame G' ss m
-    /\ (forall regs, Forall (fun v => Option.is_Some v = true) (List.map (get_reg ss.(symbolic_reg_state)) (List.map reg_index regs)))
+    /\ (forall reg, Option.is_Some (get_reg ss.(symbolic_reg_state) (reg_index reg)) = true)
     /\ gensym_dag_ok G' d'
     /\ (forall e n, eval G d e n -> eval G' d' e n).
 Proof.
@@ -2898,14 +2917,13 @@ Qed.
 
 Lemma Forall2_get_reg_of_R G d r mr regs
       (Hwide : Forall (fun reg => let '(_, _, sz) := index_and_shift_and_bitcount_of_reg reg in sz = 64%N) regs)
-      (Hknown : Forall (fun v => Option.is_Some v = true) (List.map (get_reg r) (List.map reg_index regs)))
       (Hreg : R_regs G d r mr)
-  : Forall2 (option_eq (eval_idx_Z G d))
+  : Forall2 (fun idx v => forall idx', idx = Some idx' -> eval_idx_Z G d idx' v)
             (List.map (get_reg r) (List.map reg_index regs))
-            (List.map Some (List.map (Semantics.get_reg mr) regs)).
+            (List.map (Semantics.get_reg mr) regs).
 Proof.
   induction regs as [|reg regs IH]; cbn [List.map] in *;
-    inversion Hwide; clear Hwide; inversion Hknown; clear Hknown; subst;
+    inversion Hwide; clear Hwide; subst;
     constructor; auto; clear dependent regs; [].
   assert (reg_offset reg = 0%N) by now destruct reg.
   assert (reg_index reg < length (Tuple.to_list _ r))
@@ -2921,14 +2939,14 @@ Proof.
   change (Z.of_N 64) with 64%Z.
   rewrite Z.shiftr_0_r.
   do 2 match goal with
+       | [ H : context[Tuple.nth_default ?d ?i ?l], H' : context[Tuple.nth_default ?d' ?i' ?l] |- _ ]
+         => is_evar d; unify d d'; unify i i'
        | [ H : context[Tuple.nth_default ?d ?i ?l] |- context[Tuple.nth_default ?d' ?i' ?l] ]
          => is_evar d; unify d d'; unify i i'
        end.
   cbv [R_reg] in Hreg.
   destruct Hreg as [Hreg Hreg'].
   rewrite <- Hreg'.
-  cbv [option_eq eval_idx_Z Option.is_Some] in *.
-  break_innermost_match; try discriminate; [].
   now apply Hreg.
 Qed.
 
@@ -2972,6 +2990,221 @@ Proof.
   apply IH; break_innermost_match; intros; apply Hf; cbn [List.In] in *; auto.
 Qed.
 
+Lemma load_eval_R_mem_eval G d idx idx' mem_st m' frame
+      (Hmem : R_mem frame G d mem_st m')
+      (Hload : load idx mem_st = Some idx')
+  : exists val,
+    eval_idx_Z G d idx' val.
+Proof.
+  cbv [load option_map] in *.
+  break_innermost_match_hyps; inversion_option; subst; destruct_head'_prod.
+  revert dependent m'; induction mem_st as [|m mem_st IH]; cbn [R_mem find] in *; intros.
+  all: repeat first [ progress inversion_option
+                    | progress inversion_pair
+                    | progress cbn [fst snd] in *
+                    | progress reflect_hyps
+                    | progress subst
+                    | progress specialize_by_assumption
+                    | progress break_innermost_match_hyps ].
+  all: repeat first [ progress cbv [sep R_cell64 Lift1Prop.ex1 emp eval_idx_Z] in *
+                    | progress destruct_head'_ex
+                    | progress destruct_head'_and
+                    | progress subst
+                    | now eauto ].
+Qed.
+
+Lemma load_eval_R_mem_eval_Forall2 G d idxs l n z mem_st m' frame l1
+      (Hmem : R_mem frame G d mem_st m')
+      (Hl : Forall2 (eval_idx_Z G d) l
+                    (List.map (fun i => Z.land (z + 8 * Z.of_nat i) (Z.ones 64))
+                              (seq 0 n)))
+      (Hmem_all : Option.List.lift (List.map (fun a => load a mem_st) idxs) = Some l1)
+  : exists vals,
+    Forall2 (eval_idx_Z G d) l1 vals.
+Proof.
+  revert dependent l1.
+  induction idxs as [|idx idxs IH],
+      l1 as [|x xs];
+    try specialize (IH xs); intros.
+  all: repeat first [ progress cbn [List.map fold_right] in *
+                    | progress cbv [Crypto.Util.Option.bind Option.List.lift] in *
+                    | progress inversion_option
+                    | progress inversion_list
+                    | progress destruct_head'_ex
+                    | progress destruct_head'_and
+                    | progress specialize_by reflexivity
+                    | progress subst
+                    | progress break_match_hyps
+                    | match goal with
+                      | [ H : load _ _ = Some _ |- _ ] => eapply load_eval_R_mem_eval in H; [ | eassumption ]
+                      end
+                    | now eexists nil; eauto
+                    | now eexists (_ :: _); eauto ].
+Qed.
+
+Definition R_regs_preserved_v rn (m : Semantics.reg_state)
+  := Z.land (Tuple.nth_default 0%Z rn m) (Z.ones 64).
+
+Definition R_regs_preserved G d (m : Semantics.reg_state) rs rs'
+  := forall rn idx, get_reg rs' rn = Some idx -> exists idx', get_reg rs rn = Some idx' /\ let v := R_regs_preserved_v rn m in eval_idx_Z G d idx' v -> eval_idx_Z G d idx v.
+
+Global Instance R_regs_preserved_Reflexive G d m : Reflexive (R_regs_preserved G d m) | 100.
+Proof. intro; cbv [R_regs_preserved]; eauto. Qed.
+
+Lemma R_regs_subsumed_get_reg_same_eval G d rs rs' rm
+      (H : R_regs G d rs rm)
+      (H_impl : R_regs_preserved G d rm rs rs')
+  : R_regs G d rs' rm.
+Proof.
+  cbv [R_regs get_reg R_regs_preserved R_regs_preserved_v] in *.
+  rewrite @Tuple.fieldwise_to_list_iff, @Forall2_forall_iff_nth_error in *.
+  intro i; specialize (H i); specialize (H_impl i).
+  rewrite <- !@Tuple.nth_default_to_list in *.
+  cbv [nth_default option_eq] in *.
+  repeat first [ progress destruct_head'_and
+               | progress destruct_head'_ex
+               | rewrite @Tuple.length_to_list in *
+               | progress cbv [R_reg eval_idx_Z] in *
+               | progress break_innermost_match
+               | progress break_innermost_match_hyps
+               | now auto
+               | progress intros
+               | progress subst
+               | match goal with
+                 | [ H : nth_error _ _ = None |- _ ] => apply nth_error_error_length in H
+                 | [ H : ?i >= ?n, H' : context[nth_error (Tuple.to_list ?n _) ?i] |- _ ]
+                   => rewrite nth_error_length_error in H' by now rewrite Tuple.length_to_list; lia
+                 | [ H : forall x, Some _ = Some x -> _ |- _ ]
+                   => specialize (H _ eq_refl)
+                 | [ H : ?x = ?y, H' : context[?y] |- _ ] => is_var x; rewrite <- H in H'
+                 end
+               | apply conj; auto; [] ].
+Qed.
+
+Lemma R_regs_preserved_set_reg G d rs rs' ri rm v
+      (H : R_regs_preserved G d rm rs rs')
+      (H_same : (ri < 16)%nat -> exists idx, get_reg rs ri = Some idx /\ let v' := R_regs_preserved_v ri rm in eval_idx_Z G d idx v' -> eval_idx_Z G d v v')
+  : R_regs_preserved G d rm rs (set_reg rs' ri v).
+Proof.
+  cbv [R_regs_preserved] in *.
+  intros rn idx; specialize (H rn).
+  rewrite get_reg_set_reg_full; intro.
+  repeat first [ progress break_innermost_match_hyps
+               | progress inversion_option
+               | progress subst
+               | progress destruct_head'_and
+               | progress destruct_head'_or
+               | progress destruct_head'_ex
+               | progress specialize_by_assumption
+               | progress specialize_by lia
+               | rewrite @Bool.andb_true_iff in *
+               | rewrite @Bool.andb_false_iff in *
+               | solve [ eauto ]
+               | progress reflect_hyps
+               | match goal with
+                 | [ H : forall v, ?k = Some v -> _, H' : ?k = Some _ |- _ ]
+                   => specialize (H _ H')
+                 end ].
+Qed.
+
+Lemma R_regs_preserved_fold_left_set_reg_index {T} G d rs rs' rm (r_idxs : list (_ * (_ + _ * T)))
+      (H : R_regs_preserved G d rm rs rs')
+      (H_same : Forall (fun '(r, v) => let v := match v with inl v => v | inr (v, _) => v end in exists idx, get_reg rs (reg_index r) = Some idx /\ let v' := R_regs_preserved_v (reg_index r) rm in eval_idx_Z G d idx v' -> eval_idx_Z G d v v') r_idxs)
+  : R_regs_preserved
+      G d rm
+      rs
+      (fold_left (fun rst '(r, idx')
+                  => set_reg rst (reg_index r)
+                             match idx' with
+                             | inl idx' => idx'
+                             | inr (base_idx', idxs') => base_idx'
+                             end)
+                 r_idxs rs').
+Proof.
+  revert dependent rs'; induction r_idxs as [|[r v] r_idxs IH]; cbn [fold_left];
+    inversion_one_head Forall; auto; intros; [].
+  apply IH; clear IH; auto; [].
+  apply R_regs_preserved_set_reg; auto.
+Qed.
+
+Lemma Semantics_get_reg_eq_nth_default_of_R_regs G d ss ms r
+      (Hsz : reg_size r = 64%N)
+      (HR : R_regs G d ss ms)
+  : Semantics.get_reg ms r = Tuple.nth_default 0%Z (reg_index r) (ms : Semantics.reg_state).
+Proof.
+  assert (Hro : reg_offset r = 0%N) by now revert Hsz; clear; cbv; destruct r; lia.
+  cbv [R_regs R_reg] in HR.
+  rewrite Tuple.fieldwise_to_list_iff, Forall2_forall_iff_nth_error in HR.
+  specialize (HR (reg_index r)).
+  cbv [Semantics.get_reg index_and_shift_and_bitcount_of_reg].
+  rewrite Hro, Hsz; change (Z.of_N 0) with 0%Z; change (Z.of_N 64) with 64%Z.
+  rewrite Z.shiftr_0_r, <- Tuple.nth_default_to_list; cbv [nth_default option_eq] in *.
+  break_innermost_match_hyps; break_innermost_match; inversion_option; destruct_head'_and; try congruence; try tauto.
+Qed.
+
+Lemma Semantics_get_reg_eq_nth_default_of_R frame G ss ms r
+      (Hsz : reg_size r = 64%N)
+      (HR : R frame G ss ms)
+  : Semantics.get_reg ms r = Tuple.nth_default 0%Z (reg_index r) (ms : Semantics.reg_state).
+Proof.
+  destruct ss, ms; eapply Semantics_get_reg_eq_nth_default_of_R_regs; try eassumption; apply HR.
+Qed.
+
+Lemma Forall2_R_regs_preserved_same_helper G d reg_available idxs m rs
+      (Hreg_wide_enough
+        : Forall
+            (fun reg : REG =>
+               let
+                 '(_, _, sz) := index_and_shift_and_bitcount_of_reg reg in
+               sz = 64%N) reg_available)
+      (H : Forall2 (fun (idx' : idx + idx * list idx) v
+                    => match idx' with
+                       | inl idx' => eval_idx_Z G d idx' (Z.land v (Z.ones 64))
+                       | inr (base', _) => eval_idx_Z G d base' (Z.land v (Z.ones 64))
+                       end)
+                   idxs (firstn (List.length idxs) (get_asm_reg m reg_available)))
+      (HR : R_regs G d rs m)
+      (Hex : forall n r, (n < List.length idxs)%nat -> nth_error reg_available n = Some r -> exists idx, get_reg rs (reg_index r) = Some idx)
+  : Forall (fun '(r, v)
+            => let v := match v with inl v => v | inr (v, _) => v end in
+               exists idx, get_reg rs (reg_index r) = Some idx
+                           /\ let v' := R_regs_preserved_v (reg_index r) m in eval_idx_Z G d idx v' -> eval_idx_Z G d v v')
+           (List.combine reg_available idxs).
+Proof.
+  cbv [get_asm_reg] in *.
+  rewrite firstn_map, Forall2_map_r_iff in H.
+  apply Forall2_flip in H.
+  rewrite Forall2_forall_iff_nth_error in H.
+  rewrite @Forall_forall in *.
+  intros [r ?] H'; apply In_nth_error_value in H'.
+  specialize (Hreg_wide_enough r).
+  specialize (fun v pf => Hreg_wide_enough (nth_error_In _ v pf)).
+  destruct H' as [n H'].
+  specialize (H n).
+  rewrite ListUtil.nth_error_firstn in H.
+  rewrite nth_error_combine in H'.
+  cbv [option_eq] in H.
+  cbv [R_regs_preserved_v].
+  repeat first [ progress break_innermost_match_hyps
+               | progress inversion_option
+               | progress subst
+               | progress inversion_pair
+               | progress cbv [index_and_shift_and_bitcount_of_reg] in *
+               | solve [ eauto ]
+               | match goal with
+                 | [ H : (forall reg, Option.is_Some (get_reg ?s (reg_index reg)) = true)
+                     |- context[get_reg ?s (reg_index ?ri)] ]
+                   => generalize (H ri); cbv [Option.is_Some]; break_innermost_match;
+                      try congruence
+                 | [ H : forall v, nth_error ?ls v = Some _ -> _ |- _ ]
+                   => specialize (H _ ltac:(eassumption))
+                 end ].
+  all: specialize (Hex _ _ ltac:(eassumption) ltac:(eassumption)).
+  all: destruct_head'_ex.
+  all: erewrite <- Semantics_get_reg_eq_nth_default_of_R_regs by eassumption.
+  all: eauto.
+Qed.
+
 Import Coq.Strings.String.
 Import Coq.Lists.List.
 Import Crypto.Util.Option.
@@ -2999,7 +3232,33 @@ Lemma Forall2_rets_of_R_mem {A} G frame d mem_st m' idxs base_len_base_vals rets
     TODO "Forall2_rets_of_R_mem runtime_rets R_mem postcondition"%string
     /\ Forall2 (eval_idx_or_list_idx G d) rets runtime_rets.
 Proof.
-Admitted.
+  revert dependent idxs; revert base_len_base_vals.
+  induction rets as [|ret rets IH],
+      base_len_base_vals as [|base_len_base_val base_len_base_vals],
+        idxs as [|idx idxs];
+    try specialize (IH base_len_base_vals idxs).
+  all: repeat first [ progress cbn [List.map fold_right]
+                    | progress cbv [Option.List.lift Crypto.Util.Option.bind option_map] in *
+                    | progress intros
+                    | progress subst
+                    | progress destruct_head'_ex
+                    | progress destruct_head'_and
+                    | progress inversion_option
+                    | progress inversion_list
+                    | progress specialize_by_assumption
+                    | progress specialize_by reflexivity
+                    | match goal with
+                      | [ H : Forall2 _ (_ :: _) _ |- _ ] => inversion H; clear H
+                      | [ H : Forall2 _ nil _ |- _ ] => inversion H; clear H
+                      | [ H : fold_right _ (Some nil) (List.map (fun a => load a _) _) = Some _ |- _ ]
+                        => eapply load_eval_R_mem_eval_Forall2 in H; [ | eassumption .. ]
+                      end
+                    | break_innermost_match_step
+                    | break_innermost_match_hyps_step
+                    | progress break_match_hyps
+                    | now eexists nil; split; auto using todo
+                    | now eexists (inr _ :: _); eauto ].
+Qed.
 
 Local Ltac saturate_lengths_step :=
   match goal with
@@ -3090,11 +3349,23 @@ Proof.
                  | [ x := ?y |- _ ] => subst x
                  end ].
   cbv [R_runtime_input] in HR; repeat (destruct_head'_ex; destruct_head'_and).
-  destruct (init_symbolic_state_ok m G _ _ ltac:(eassumption) ltac:(eassumption) eq_refl) as [G1 ?]; destruct_head'_and.
+  let HR := lazymatch goal with HR : sep _ _ (machine_mem_state m) |- _ => HR end in
+  destruct (init_symbolic_state_ok m G _ _ ltac:(eassumption) ltac:(eassumption) HR) as [G1 ?]; destruct_head'_and.
   let debug_run tac := tac () in
+  let in_evars_do tac :=
+    let do_with ev :=
+      let H := fresh in
+      pose ev as H;
+      (instantiate (1:=ltac:(progress tac)) in (value of H)); subst H in
+    repeat match goal with
+           | [ H : context[?ev] |- _ ] => is_evar ev; do_with ev
+           | [ H := context[?ev] |- _ ] => is_evar ev; do_with ev
+           | [ |- context[?ev] ] => is_evar ev; do_with ev
+           end in
   repeat first [ progress destruct_head'_ex
                | progress destruct_head'_and
                | progress cbn [update_dag_with Symbolic.dag_state Symbolic.symbolic_flag_state Symbolic.symbolic_mem_state Symbolic.symbolic_reg_state] in *
+               | solve [ auto ]
                | match reverse goal with
                  | [ H : build_inputs _ _ = _ |- exists m' : machine_state, _ ]
                    => debug_run ltac:(fun _ => idtac "build_inputs start");
@@ -3157,34 +3428,19 @@ Proof.
                       [ | clear H; try assumption .. ];
                       [
                       | lazymatch goal with
-                        | [ |- Forall2 (option_eq (eval_idx_Z _ _))
+                        | [ |- Forall2 (fun idx v => forall idx', idx = Some idx' -> eval_idx_Z _ _ idx' v)
                                        (List.map (get_reg _) (List.map reg_index _))
-                                       (List.map Some _) ]
+                                       _ ]
                           => destruct_head' symbolic_state; cbn [Symbolic.symbolic_reg_state Symbolic.dag_state] in *; subst;
-                             idtac "TODO: this is actually wrong, because we're not guaranteed that the symeval won't clear registers";
                              eapply Forall2_get_reg_of_R;
                              [ lazymatch goal with
                                | [ |- R_regs _ _ _ _ ]
-                                 => match goal with H : R _ _ _ _ |- _ => try eapply H end
-                               | [ |- Forall (fun v => Option.is_Some v = true)
-                                             (List.map (get_reg _) _) ]
-                                 => repeat
-                                      match goal with
-                                      | [ |- Forall (fun v => Option.is_Some v = true)
-                                                    (List.map (get_reg (set_reg _ _ _)) _) ]
-                                        => apply reg_all_set_set_reg
-                                      | [ |- Forall (fun v => Option.is_Some v = true)
-                                                    (List.map (get_reg (fold_left _ _ _)) _) ]
-                                        => apply reg_all_set_fold_left; intros
-                                      | [ |- context[let '(_, _) := ?x in _] ]
-                                        => is_var x; destruct x
-                                      | [ |- Forall (fun v => Option.is_Some v = true)
-                                                    (List.map (get_reg _) _) ]
-                                        => solve [ auto | assumption ]
-                                      end
+                                 => try match goal with H : R _ _ _ _ |- _ => eapply H end
                                | _ => idtac
                                end .. ];
-                             try assumption
+                             repeat first [ assumption
+                                          | reflexivity
+                                          | rewrite map_length ]
                         | [ |- gensym_dag_ok _ _ ] => eassumption
                         | _ => idtac
                         end .. ];
@@ -3194,8 +3450,12 @@ Proof.
                                       (List.map (Semantics.get_reg _) _) ]
                           => apply get_reg_bounded
                         | _ => idtac
-                        end .. ];
-                      [ | match goal with |- ?G => idtac "TODO" G end .. ];
+                        end;
+                        repeat first [ assumption
+                                     | reflexivity
+                                     | rewrite map_length ] .. ];
+                      (* some of these will be resolved later *)
+                      [ | debug_run ltac:(fun _ => match goal with |- ?G => idtac "TODO" G end) .. ];
                       debug_run ltac:(fun _ => idtac "get callee_saved_registers end")
                  | [ H : SymexLines _ _ = Success _ |- exists m' : machine_state, _ ]
                    => debug_run ltac:(fun _ => idtac "SymexLines start");
@@ -3207,7 +3467,29 @@ Proof.
                                | [ H : R _ ?G ?s _ |- _ ]
                                  => unique assert (gensym_dag_ok G s) by (destruct s; apply H)
                                end
-                      | clear H .. ];
+                      | clear H;
+                        lazymatch goal with
+                        | [ H : R _ _ _ ?m |- R ?frame' _ _ ?m' ]
+                          => move H at bottom; unify frame frame'; unify m m'; cbv [update_dag_with R];
+                             destruct_head' symbolic_state;
+                             cbn [update_dag_with Symbolic.dag_state Symbolic.symbolic_flag_state Symbolic.symbolic_mem_state Symbolic.symbolic_reg_state] in *;
+                             subst;
+                             destruct_head'_and;
+                             repeat first [ solve [ auto ]
+                                          | progress cbn [update_dag_with Symbolic.dag_state Symbolic.symbolic_flag_state Symbolic.symbolic_mem_state Symbolic.symbolic_reg_state] in *
+                                          | progress subst
+                                          | eapply R_flags_subsumed; [ eassumption | now eauto ]
+                                          | match goal with
+                                            | [ |- _ /\ _ ] => split
+                                            | [ |- R_flags _ _ _ _ ]
+                                              => progress
+                                                   (cbv [R update_dag_with] in *;
+                                                    destruct_head'_and)
+                                            | [ |- gensym_dag_ok _ _ ]
+                                              => progress destruct_head' symbolic_state
+                                            end ]
+                        | _ => idtac
+                        end .. ];
                       [ | match goal with |- ?G => idtac "TODO" G end .. ];
                       debug_run ltac:(fun _ => idtac "SymexLines end")
                  | [ H : LoadOutputs _ _ _ = _ |- exists runtime_rets : list (Z + list Z), _ ]
@@ -3222,16 +3504,96 @@ Proof.
                         end .. ];
                       [];
                       debug_run ltac:(fun _ => idtac "LoadOutputs end")
-                 end ].
-  eexists.
-  repeat (apply conj; eauto 10; []).
-  all: let do_with ev := (let H := fresh in pose ev as H; instantiate (1:=ltac:(progress (repeat match goal with H : symbolic_state |- _ => clear dependent H | [ H : list Z |- _ ] => clear dependent H end))) in (value of H); subst H) in
-       repeat match goal with
-              | [ H : context[?ev] |- _ ] => is_evar ev; do_with ev
-              | [ H := context[?ev] |- _ ] => is_evar ev; do_with ev
-              | [ |- context[?ev] ] => is_evar ev; do_with ev
-              end.
-  move rets at bottom.
+                 | [ H : Some ?rets = Option.List.lift (List.map (fun idxs => match idxs with inr idxs' => option_map inr (Option.List.lift (List.map (fun a => load a _) idxs')) | inl _ => _ end) _) |- exists runtime_rets : list (Z + list Z), _ ]
+                   => debug_run ltac:(fun _ => idtac "Forall2_rets_of_R_mem start");
+                      eapply Forall2_rets_of_R_mem in H;
+                      [ destruct H as [runtime_rets H]; exists runtime_rets
+                      | clear H;
+                        lazymatch goal with
+                        | [ |- Forall2 _ _ _ ] => eassumption
+                        | [ |- R_mem _ _ _ _ _ ]
+                          => eapply R_mem_subsumed;
+                             lazymatch goal with
+                             | [ H : R ?frame ?G ?ss ?ms |- R_mem ?frame' ?G' ?d ?ss' ?ms' ]
+                               => let unif_or_eq x y := first [ unify x y | let H := fresh in assert (H : y = x) by congruence; rewrite H ] in
+                                  unif_or_eq frame frame'; unif_or_eq G G';
+                                  unif_or_eq (Symbolic.dag_state ss) d;
+                                  unif_or_eq (Symbolic.symbolic_mem_state ss) ss';
+                                  unif_or_eq (machine_mem_state ms) ms';
+                                  cbv [R] in H;
+                                  destruct_head' symbolic_state; apply H
+                             | _ => eauto
+                             end
+                        end .. ];
+                      [];
+                      debug_run ltac:(fun _ => idtac "Forall2_rets_of_R_mem end")
+                 | [ H : R _ _ (update_dag_with (init_symbolic_state _) _) ?m
+                     |- R_regs _ _ (set_reg (fold_left _ _ (Symbolic.symbolic_reg_state (init_symbolic_state _))) _ _) ?m' ]
+                   => debug_run ltac:(fun _ => idtac "R => R_regs set_reg start");
+                      in_evars_do ltac:(destruct_head' symbolic_state; cbn [Symbolic.symbolic_reg_state Symbolic.dag_state] in * );
+                      eapply R_regs_subsumed_get_reg_same_eval;
+                      [ eapply R_regs_subsumed;
+                        [ apply H | now eauto ]
+                      | let finish_some_reg _ :=
+                          cbv [R_regs_preserved_v];
+                          match goal with
+                          | [ H : (forall reg, Option.is_Some (get_reg ?s (reg_index reg)) = true)
+                              |- context[get_reg ?s (reg_index ?ri)] ]
+                            => generalize (H ri); cbv [Option.is_Some]; break_innermost_match;
+                               try congruence
+                          end;
+                          eauto using lift_eval_idx_Z_impl in
+                        let rec do_stuff _
+                          := lazymatch goal with
+                             | [ |- R_regs_preserved _ _ _ ?x ?x ] => reflexivity
+                             | [ |- R_regs_preserved _ _ _ _ (set_reg _ _ _) ]
+                               => apply R_regs_preserved_set_reg;
+                                  [ do_stuff ()
+                                  | solve [ intros; finish_some_reg () ] ]
+                             | [ |- R_regs_preserved _ _ _ _ (fold_left _ _ _) ]
+                               => apply R_regs_preserved_fold_left_set_reg_index;
+                                  [ do_stuff ()
+                                  | lazymatch goal with
+                                    | [ H : Forall2 _ ?x (firstn (List.length ?x) (get_asm_reg _ ?reg_available))
+                                        |- Forall _ (List.combine ?reg_available ?x) ]
+                                      => eapply Forall2_R_regs_preserved_same_helper;
+                                         lazymatch goal with
+                                         | [ |- Forall2 _ x (firstn (List.length x) (get_asm_reg _ reg_available)) ]
+                                           => eapply Forall2_weaken; [ | exact H ];
+                                              cbv beta; intros *; break_innermost_match;
+                                              intros; destruct_head'_and; eauto using lift_eval_idx_Z_impl
+                                         | [ H : R _ _ _ _ |- R_regs _ _ _ _ ] => eapply R_regs_subsumed; [ apply H | eauto ]
+                                         | _ => first [ assumption
+                                                      | intros; finish_some_reg ()
+                                                      | idtac ]
+                                         end
+                                    end ]
+                             end in
+                        do_stuff () ];
+                      [ match goal with |- ?G => idtac "TODO" G end .. ];
+                      debug_run ltac:(fun _ => idtac "R => R_regs set_reg end")
+                 end
+               | progress repeat (apply conj; eauto 10; []) ].
+  all: cbn [update_dag_with Symbolic.dag_state Symbolic.symbolic_flag_state Symbolic.symbolic_mem_state Symbolic.symbolic_reg_state] in *.
+  (* remaining goals:
+============================
+  R_runtime_output frame runtime_rets
+    (type_spec_of_runtime (word_args_to_Z_args word_runtime_inputs))
+    (Datatypes.length x) stack_base asm_args_out asm_args_in callee_saved_registers
+    runtime_callee_saved_registers m'
+
+goal 2 (ID 12848) is:
+ R_mem frame G_final dag_state1
+   (rev (List.combine x4 x5) ++
+    rev
+      (flat_map
+         (fun pat : (idx + idx * list idx) * (idx + list idx) =>
+          match pat with
+          | (inl _, _) => []
+          | (inr (_, addrs'), inl _) => []
+          | (inr (_, addrs'), inr items) => List.combine addrs' items
+          end) (List.combine x3 (l4 ++ inputs))) ++ init_symbolic_state d) m
+   *)
 Admitted.
 
 Theorem symex_asm_func_correct
